pcuic/theories/PCUICUnivSubstitution.v
@@ -133,7 +133,7 @@ Lemma subst_equal_inst_global_inst Σ Re gr napp :
                                     (subst_instance_instance u2 u).
 Proof.
   intros reflRe hRe u u1 u2 Ru1u2.
-  unfold R_global_instance.
+  unfold R_global_instance, R_opt_variance.
   destruct global_variance as [v|]; auto using subst_equal_inst_inst.
   induction u in v |- *; cbnr; try now constructor.
   - destruct v; simpl; auto.
@@ -843,7 +843,7 @@ Lemma precompose_subst_instance_global Σ Re Rle gr napp u i i' :
   <~> R_global_instance Σ (precompose Re (subst_instance_univ u)) 
     (precompose Rle (subst_instance_univ u)) gr napp i i'.
 Proof.
-  unfold R_global_instance, subst_instance_instance.
+  unfold R_global_instance, R_opt_variance, subst_instance_instance.
   destruct global_variance as [v|]; eauto using precompose_subst_instance_instance.
   induction i in i', v |- *; destruct i', v; simpl; try split; auto.
   - destruct (IHi i' []). intros; auto.
